Core/Metatheory/Preservation.lean
@@ -3,6 +3,9 @@ import Core.Term
 import Core.Reduction
 import Core.Typing
 
+import Core.Metatheory.Substitution
+import Core.Metatheory.Rename
+
 open LeanSubst
 
 
@@ -10,6 +13,9 @@ theorem refl_spine_lemma :
   OpenVarVal G n sp ->
   ¬ (G&Δ, Γ ⊢ (g#n).apply sp : (A ~[K]~ B)) := by
 intro h j
+generalize tdef : (g#n).apply sp = t at *
+generalize Tdef : (A ~[K]~ B) = T at *
+-- induction j <;> simp at *
 
 sorry
 
@@ -24,46 +30,310 @@ case refl =>
 case choice t1 t2 _ _ ih1 ih2 =>
   cases j; apply Or.inr;  exists t1; exists t2
 case app ih =>
-
   sorry
 
-theorem well_typed_values_do_not_reduce :
-  G&Δ, Γ ⊢ t : T ->
-  Value G t -> ¬ G ⊢ t ~> t' := by
-intro j h r
-induction h generalizing T
-case app => sorry
-case choice ih1 ih2 => sorry
-case lam => sorry
-case lamt => sorry
-case refl => sorry
 
-theorem reduct_not_value :
-  G ⊢ t ~> t' -> ¬ Value G t := by sorry
+theorem var_val_sound :
+  t.spine = some (x, sp) ->
+  is_stable x G ∨ OpenVarVal G x sp ->
+  ∀ t', ¬ G ⊢ t ~> t' := by
+intro h1 h2 t' r
+induction t generalizing x sp G
+any_goals (simp [Term.spine] at h1)
+case global =>
+  cases r;
+  case _ h2' _ _ _ _ _ h _ =>
+    simp [is_stable] at h2;   simp [Term.spine] at h
+    rcases h1 with ⟨e1, e2⟩; cases e1; cases e2; simp at *
+    rcases h with ⟨e1, e2⟩; cases e1; cases e2; simp at *
+    cases h2
+    case _ h =>
+      have lem := lookup_entry_openm_exists h2';
+      rcases lem with ⟨_, _, lem⟩
+      simp [is_ctor, is_instty] at h; rw[lem] at h
+      simp at h; simp [Entry.is_ctor, Entry.is_instty] at h
+    case _ h3 _ _ _ _ h =>
+      simp [OpenVarVal] at h;
+      rcases h with ⟨_, h⟩
+      replace h := h _ h3; omega
+  sorry
+case ctor1 v _ ih =>
+  cases v <;> simp [Term.spine] at h1
+  rw[Option.bind_eq_some_iff] at h1; rcases h1 with ⟨_, h1, h2⟩; cases h2
+  cases r
+  all_goals (try simp [Term.spine] at h1)
+  case _ h _ =>
+    simp [Term.spine] at h; symm at h;
+    rw[Option.bind_eq_some_iff] at h; rcases h with ⟨_, h, e⟩; cases e
+    rw[h1] at h; cases h
+    simp [is_stable] at h2; case _ h2' _ _ _ _ _ =>
+    cases h2
+    case _ w _ _ _ _ _ _ _ _ _ h =>
+      have lem := @is_stable_implies_not_is_openm w.fst G (by simp [is_stable]; assumption)
+      apply lem h2'
+    case _ h3 _ _ h4 _ h =>
+      simp [OpenVarVal] at h
+      rcases h with ⟨_, h⟩
+      replace h :=  h _ h3
+      simp at h4; omega
+  case _ h => sorry
+  sorry
+case ctor2 v f _ ih1 ih2 =>
+  cases v <;> simp at *
+  all_goals (try simp [Term.spine] at h1)
+  case _ b =>
+    cases b <;> simp at *
+    case closed =>
+      cases r <;> try simp [Term.spine] at h1
+      case _ h _ =>
+        simp [Term.spine] at h; symm at h;
+        rw[Option.bind_eq_some_iff] at h; rcases h with ⟨w, h, e⟩; cases e
+        rcases h1 with ⟨_, e, h1⟩
+        rw[h1] at h; cases h
+        simp [is_stable] at h2; case _ h2' _ _ _ _ _ =>
+        cases h2
+        case _ w _ _ _ _ _ _ _ _ _ h =>
+          have lem := @is_stable_implies_not_is_openm x G (by simp [is_stable]; assumption)
+          apply lem h2'
+        case _ h3 _ _ h4 _ h =>
+          simp [OpenVarVal] at h
+          rcases h with ⟨_, h⟩
+          replace h :=  h _ h3
+          simp at h4; rw[e] at h; simp at h; omega
+      case _ => sorry
+      all_goals (try case _ h _ => simp at h)
+      case _ h => sorry -- simp at h
+      sorry
+    case «open» =>
+      cases r <;> try simp [Term.spine] at h1
+      case _ h _ =>
+        simp [Term.spine] at h; symm at h;
+        rw[Option.bind_eq_some_iff] at h; rcases h with ⟨w, h, e⟩; cases e
+        rcases h1 with ⟨_, e, h1⟩
+        rw[h1] at h; cases h
+        simp [is_stable] at h2; case _ h2' _ _ _ _ _ =>
+        cases h2
+        case _ w _ _ _ _ _ _ _ _ _ h =>
+          have lem := @is_stable_implies_not_is_openm x G (by simp [is_stable]; assumption)
+          apply lem h2'
+        case _ h3 _ _ h4 _ h =>
+          simp [OpenVarVal] at h
+          rcases h with ⟨_, h⟩
+          replace h :=  h _ h3
+          simp at h4; rw[e] at h; simp at h; omega
+      case _ => sorry
+      case _ h _ => sorry
+      sorry
+      sorry
+      sorry
 
-theorem preservation :
+
+theorem value_sound :
+  Value G t ->
+  t ≠ `0 ∧ ∀ t', ¬ G ⊢ t ~> t' := by
+intro h; induction h
+case _ =>
+  simp at *
+  constructor;
+  intro h; case _ tnf _ _ _ _  => rw[h] at tnf; simp [Term.spine] at tnf
+  case _ tnf _ _ h _ =>
+  apply var_val_sound (Eq.symm tnf); assumption
+all_goals (
+  case _ =>
+  apply And.intro; simp
+  intro t' r;
+  cases r <;> simp at *
+  try case right.ctor2_congr1 ih1 ih2 _ r _ =>
+      cases ih1; case _ h1 h2 =>
+      apply h2 _ r
+  try case right.ctor2_congr2 ih1 ih2 _ r _ =>
+      cases ih2; case _ h1 h2 =>
+      apply h2 _ r
+  try case _ h _ _ => simp [Term.spine] at h
+  try case _ h => simp [Term.spine] at h
+)
+
+theorem reduction_sound :
+  G ⊢ t ~> t' -> ¬ Value G t := by
+intro r v
+have lem := value_sound v
+rcases lem with ⟨_ , lem⟩
+apply lem t' r
+
+theorem instance_type_preservation :
+  ⊢ G ->
+  G&Δ, Γ ⊢ g#x : T ->
+  instances x G = is ->
+  ∀ t ∈ is, G&Δ, Γ ⊢ t : T := by
+intro wf j h t t_in_is
+sorry
+
+theorem preservation_lemma :
+  Δ = [] -> Γ = [] ->
   G&Δ, Γ ⊢ t : T ->
   G ⊢ t ~> t' ->
   G&Δ, Γ ⊢ t' : T  := by
-intro j h
-induction j
-case var => sorry
+intro e1 e2 j h
+induction j generalizing t' <;> simp at *
+case var h' _ => rw[e2] at h'; simp at h'
+all_goals (cases e1; cases e2)
+all_goals (try simp at *)
 case global => sorry
-case mtch => sorry
-case guard => sorry
-case lam => sorry
+  -- cases h; simp at *;
+  -- case _ h _ _ _ =>
+  -- cases h
+  -- sorry
+case mtch =>
+  sorry
+case guard =>
+  cases h
+  case guard_matched => sorry
+  case guard_missed => sorry
+  all_goals (try case _ h => simp [Term.spine] at h)
+  all_goals (try case _ h _ => simp [Term.spine] at h)
+  all_goals (try case _ h _ _ => simp at h)
+  · sorry
+  · sorry
+  · constructor
+    sorry
+    sorry
+    sorry
+    sorry
+
 case app => sorry
-case lamt => sorry
 case appt => sorry
-case cast => sorry
-case refl => sorry
-case sym => sorry
-case seq => sorry
+case lam =>
+  cases h;
+  case _ h _ => cases h
+  case _ h => simp [Term.spine] at h
+case lamt =>
+  cases h;
+  case _ h _ => cases h
+  case _ h => simp [Term.spine] at h
+  all_goals (case _ h _ => simp at h)
+case cast tj cj _ ih =>
+  cases h
+  all_goals (try case _ h => simp [Term.spine] at h)
+  all_goals (try case _ h _ => simp [Term.spine] at h)
+  all_goals (try case _ h _ _ => simp at h)
+  case _ => cases cj; assumption
+  case _ t _ c _ _ _ t' h cr =>
+    simp at *; replace ih := ih cr
+    constructor; assumption; assumption
+  case _ =>
+    cases cj; case _ cj =>
+    cases cj; constructor; assumption
+  case _ =>
+    cases cj; case _ cj _ _ =>
+    cases cj;
+    apply Typing.choice
+    assumption
+    constructor; assumption; assumption
+    constructor; assumption; assumption
+
+case refl =>
+  cases h
+  case _ h _ => cases h
+  case _ h => simp [Term.spine] at h
+case sym =>
+  cases h;
+  all_goals (try case _ h => simp [Term.spine] at h)
+  all_goals (try case _ h _ => simp [Term.spine] at h)
+  all_goals (try case _ h _ _ => simp at h)
+
+  case _ h _ => cases h; constructor; assumption
+  case _ ih t' r => replace ih := ih r; constructor; assumption
+  case _ j _ =>
+    cases j; case _ j =>
+    cases j; case _ K _ _ _ _ _ =>
+    apply Typing.zero (K := ★)
+    constructor; assumption; assumption
+  case _ j ih =>
+    cases j; case _ j _ _ =>
+    cases j
+    apply Typing.choice
+    constructor; assumption; assumption
+    constructor; assumption
+    constructor; assumption
+case seq =>
+  cases h
+  all_goals (try case _ h => simp [Term.spine] at h)
+  all_goals (try case _ h _ => simp [Term.spine] at h)
+  all_goals (try case _ h _ _ => simp at h)
+  sorry
+  sorry
+  sorry
+  sorry
+  sorry
+  sorry
+  sorry
 case appc => sorry
 case arrowc => sorry
 case fst => sorry
 case snd => sorry
-case allc => sorry
-case apptc => sorry
-case zero => cases h; simp at *; sorry
-case choice => sorry
+case allc =>
+  cases h
+  all_goals (try case _ h => simp [Term.spine] at h)
+  all_goals (try case _ h _ => simp [Term.spine] at h)
+  all_goals (try case _ h _ _ => simp [Term.spine] at h)
+  case _ h => cases h; case _ h => constructor; constructor; assumption
+  case _ h _ =>
+    simp at h
+    constructor; simp;
+    sorry -- where did my induction hypothesis go?
+    sorry
+  case _ h =>
+    cases h; case _ h =>
+    cases h;
+    constructor; constructor; sorry; sorry
+  case _ h =>
+    cases h
+    constructor
+    constructor;
+    sorry;
+    sorry
+    constructor; simp; assumption
+    constructor; simp; assumption
+
+case apptc =>
+  cases h
+  all_goals (try case _ h => simp [Term.spine] at h)
+  all_goals (try case _ h _ => simp [Term.spine] at h)
+  all_goals (try case _ h _ _ => simp at h)
+  case _ e1 e2 _ _ _ h1 _ h2 _ =>
+    cases h1; cases h2
+    rw[<-e1] at e2; rw[e2]; rw[e1]
+    constructor; case _ j1 _ j2 _ =>
+    cases j1; case _ j1 =>
+    have lem := Kinding.beta j1 j2
+    sorry
+  case _ => sorry
+  case _ => sorry
+  case _ => sorry
+  case _ => sorry
+  case _ => sorry
+  case _ => sorry
+
+case zero =>
+  cases h;
+  case _ h _ => cases h
+  all_goals (try case _ h => simp [Term.spine] at h)
+
+case choice =>
+  cases h
+  all_goals (try assumption)
+  all_goals (try case _ h => simp [Term.spine] at h)
+  all_goals (try case _ h _ => simp [Term.spine] at h)
+  case _ ih _ _ _ r =>
+    replace ih := ih r
+    apply Typing.choice; assumption; assumption; assumption
+  case _ ih _ _ r =>
+    replace ih := ih r
+    apply Typing.choice; assumption; assumption; assumption
+  all_goals (case _ h _ _ => simp at h)
+
+
+theorem preservation :
+  G&[], [] ⊢ t : T ->
+  G ⊢ t ~> t' ->
+  G&[], [] ⊢ t' : T  := by intro j r; apply preservation_lemma rfl rfl j r
